Refactoring type soundness proof (#31)
* remove trait/class from validation proof

* update forall notation

* apply formatter

cedar-dafny/validation/thm/soundness.dfy
@@ -34,7 +34,7 @@ module validation.thm.soundness {
 
   type Result<T> = types.Result<T>
 
-  // A value of type SemanticSoundnessProof(model,reqty,ets,acts,q,s) contains a
+  // A value of type SemanticSoundnessProof(reqty,ets,acts,q,s) contains a
   // proof (`lemma SoundToplevel` at the bottom of the file) that any
   // expression `e` typed in context (reqty, ets, acts) and evaluated under (r,s)
   // is safe according to the model, assuming the context assigns correct
@@ -43,7 +43,6 @@ module validation.thm.soundness {
   // The proofs in this file are robust to changes in the evaluator, since they
   // only depend on the abstract `model`.
   datatype SemanticSoundnessProof = SSP(
-    model: SemanticModel,
     reqty: RequestType,
     ets: EntityTypeStore,
     acts: ActionStore,
@@ -76,14 +75,14 @@ module validation.thm.soundness {
     // On input to the typechecking function, for any (e,k) in the Effects,
     // e is a record- or entity-typed expression that has key k.
     ghost predicate {:opaque} EffectsInvariant (effs: Effects) {
-      forall e, k | (e, k) in effs.effs :: model.GetAttrSafe(r,s,e,k)
+      forall e, k | (e, k) in effs.effs :: GetAttrSafe(r,s,e,k)
     }
 
     // The Effects output by the typechecking function, will satisfy
     // `EffectsInvariant` provided that the input expression is true.
     ghost predicate GuardedEffectsInvariant (e: Expr, effs: Effects)
     {
-      model.IsTrueStrong(r,s,e) ==> EffectsInvariant(effs)
+      IsTrueStrong(r,s,e) ==> EffectsInvariant(effs)
     }
 
     lemma EmptyEffectsInvariant ()
@@ -95,23 +94,23 @@ module validation.thm.soundness {
     lemma SoundLit(p: Primitive, t: Type, effs: Effects)
       decreases PrimitiveLit(p) , 0
       requires Typesafe(PrimitiveLit(p),effs,t)
-      ensures model.IsSafe(r,s,PrimitiveLit(p),t)
+      ensures IsSafe(r,s,PrimitiveLit(p),t)
       ensures getEffects(PrimitiveLit(p),effs) == Effects.empty()
     {
       assert InstanceOfType(Primitive(p),typeOfPrim(p)) by {
-        model.PrimSafeAtInferredType(p);
+        PrimSafeAtInferredType(p);
       }
 
-      assert model.SemanticSubty(typeOfPrim(p),t) by {
-        model.SubtyCompat(typeOfPrim(p),t);
+      assert SemanticSubty(typeOfPrim(p),t) by {
+        SubtyCompat(typeOfPrim(p),t);
       }
 
       assert InstanceOfType(Primitive(p),t) by {
-        model.SemSubtyTransportVal(typeOfPrim(p),t,Primitive(p));
+        SemSubtyTransportVal(typeOfPrim(p),t,Primitive(p));
       }
 
-      assert model.IsSafe(r,s,PrimitiveLit(p),t) by{
-        model.PrimSafeLift(r,s,p,t);
+      assert IsSafe(r,s,PrimitiveLit(p),t) by{
+        PrimSafeLift(r,s,p,t);
       }
     }
 
@@ -121,37 +120,37 @@ module validation.thm.soundness {
       requires InstanceOfEntityTypeStore(s,ets)
       requires InstanceOfActionStore(s,acts)
       requires Typesafe(Var(x),effs,t)
-      ensures model.IsSafe(r,s,Var(x),t)
+      ensures IsSafe(r,s,Var(x),t)
       ensures getEffects(Var(x),effs) == Effects.empty()
     {
       var t' :| getType(Var(x),effs) == t' && subty(t',t);
       assert Typechecker(ets,acts,reqty).inferVar(x) == types.Ok(t');
       match x {
         case Principal =>
-          assert model.IsSafe(r,s,Var(Principal),t') by { model.PrincipalIsSafe(r,s,t'); }
-          assert model.IsSafe(r,s,Var(Principal),t) by {
-            model.SubtyCompat(t',t);
-            model.SemSubtyTransport(r,s,Var(Principal),t',t);
+          assert IsSafe(r,s,Var(Principal),t') by { PrincipalIsSafe(r,s,t'); }
+          assert IsSafe(r,s,Var(Principal),t) by {
+            SubtyCompat(t',t);
+            SemSubtyTransport(r,s,Var(Principal),t',t);
           }
         case Action =>
-          assert model.IsSafe(r,s,Var(Action),t') by { model.ActionIsSafe(r,s,t'); }
-          assert model.IsSafe(r,s,Var(Action),t) by {
-            model.SubtyCompat(t',t);
-            model.SemSubtyTransport(r,s,Var(Action),t',t);
+          assert IsSafe(r,s,Var(Action),t') by { ActionIsSafe(r,s,t'); }
+          assert IsSafe(r,s,Var(Action),t) by {
+            SubtyCompat(t',t);
+            SemSubtyTransport(r,s,Var(Action),t',t);
           }
         case Resource =>
-          assert model.IsSafe(r,s,Var(Resource),t') by { model.ResourceIsSafe(r,s,t'); }
-          assert model.IsSafe(r,s,Var(Resource),t) by {
-            model.SubtyCompat(t',t);
-            model.SemSubtyTransport(r,s,Var(Resource),t',t);
+          assert IsSafe(r,s,Var(Resource),t') by { ResourceIsSafe(r,s,t'); }
+          assert IsSafe(r,s,Var(Resource),t) by {
+            SubtyCompat(t',t);
+            SemSubtyTransport(r,s,Var(Resource),t',t);
           }
         case Context =>
-          assert model.IsSafe(r,s,Var(Context),Type.Record(reqty.context)) by {
-            model.ContextIsSafe(r,s,Type.Record(reqty.context));
+          assert IsSafe(r,s,Var(Context),Type.Record(reqty.context)) by {
+            ContextIsSafe(r,s,Type.Record(reqty.context));
           }
-          assert model.IsSafe(r,s,Var(Context),t) by {
-            model.SubtyCompat(Type.Record(reqty.context),t);
-            model.SemSubtyTransport(r,s,Var(Context),Type.Record(reqty.context),t);
+          assert IsSafe(r,s,Var(Context),t) by {
+            SubtyCompat(Type.Record(reqty.context),t);
+            SemSubtyTransport(r,s,Var(Context),Type.Record(reqty.context),t);
           }
       }
     }
@@ -188,13 +187,13 @@ module validation.thm.soundness {
       requires InstanceOfActionStore(s,acts)
       requires EffectsInvariant(effs)
       requires Typesafe(If(e,e1,e2),effs,t)
-      ensures model.IsSafe(r,s,If(e,e1,e2),t)
+      ensures IsSafe(r,s,If(e,e1,e2),t)
       ensures GuardedEffectsInvariant(If(e,e1,e2),getEffects(If(e,e1,e2),effs))
     {
       var t' :| getType(If(e,e1,e2),effs) == t' && subty(t',t);
       assert Typechecker(ets,acts,reqty).inferIf(e,e1,e2,effs).Ok?;
       var (bt, effs1) := Typechecker(ets,acts,reqty).inferBoolType(e,effs).value;
-      assert model.IsSafe(r,s,e,Type.Bool(bt)) && GuardedEffectsInvariant(e,effs1) by {
+      assert IsSafe(r,s,e,Type.Bool(bt)) && GuardedEffectsInvariant(e,effs1) by {
         assert getType(e,effs) == Type.Bool(bt);
         assert subty(Type.Bool(bt),Type.Bool(bt));
         assert Typesafe(e,effs,Type.Bool(bt));
@@ -202,51 +201,51 @@ module validation.thm.soundness {
       }
       match bt {
         case True =>
-          assert model.IsTrue(r,s,e);
+          assert IsTrue(r,s,e);
           var (t1,effs2) := Typechecker(ets,acts,reqty).infer(e1,effs.union(effs1)).value;
           assert Typesafe(e1,effs.union(effs1),t1) by { SubtyRefl(t1); }
-          if model.IsTrueStrong(r,s,e) {
+          if IsTrueStrong(r,s,e) {
             assert EffectsInvariant(effs1);
-            assert model.IsSafe(r,s,e1,t1) && GuardedEffectsInvariant(e1,effs2) by {
+            assert IsSafe(r,s,e1,t1) && GuardedEffectsInvariant(e1,effs2) by {
               EffectsInvariantUnion(effs,effs1);
               Sound(e1,t1,effs.union(effs1));
             }
-            assert model.IsSafe(r,s,If(e,e1,e2),t') by { model.IteTrueSafe(r,s,e,e1,e2,t'); }
-            assert model.IsSafe(r,s,If(e,e1,e2),t) by {
-              model.SubtyCompat(t',t);
-              model.SemSubtyTransport(r,s,If(e,e1,e2),t',t);
+            assert IsSafe(r,s,If(e,e1,e2),t') by { IteTrueSafe(r,s,e,e1,e2,t'); }
+            assert IsSafe(r,s,If(e,e1,e2),t) by {
+              SubtyCompat(t',t);
+              SemSubtyTransport(r,s,If(e,e1,e2),t',t);
             }
             assert GuardedEffectsInvariant(If(e,e1,e2),effs1.union(effs2)) by {
-              if model.IsTrueStrong(r,s,If(e,e1,e2)) {
-                model.IteTrueStrongTrue(r,s,e,e1,e2);
+              if IsTrueStrong(r,s,If(e,e1,e2)) {
+                IteTrueStrongTrue(r,s,e,e1,e2);
                 assert EffectsInvariant(effs2);
                 EffectsInvariantUnion(effs1,effs2);
               }
             }
           } else {
-            assert model.IsSafe(r,s,If(e,e1,e2),t) by {
-              model.IteError(r,s,e,e1,e2,Type.Bool(True),t);
+            assert IsSafe(r,s,If(e,e1,e2),t) by {
+              IteError(r,s,e,e1,e2,Type.Bool(True),t);
             }
             assert GuardedEffectsInvariant(If(e,e1,e2),effs1.union(effs2)) by {
-              model.IteError(r,s,e,e1,e2,Type.Bool(True),Type.Bool(True));
-              assert !model.IsTrueStrong(r,s,If(e,e1,e2));
+              IteError(r,s,e,e1,e2,Type.Bool(True),Type.Bool(True));
+              assert !IsTrueStrong(r,s,If(e,e1,e2));
             }
           }
         case False =>
-          assert model.IsFalse(r,s,e);
+          assert IsFalse(r,s,e);
           var (t2,effs2) := Typechecker(ets,acts,reqty).infer(e2,effs).value;
           assert Typesafe(e2,effs,t2) by { SubtyRefl(t2); }
-          assert model.IsSafe(r,s,e2,t2) && GuardedEffectsInvariant(e2,effs2) by {
+          assert IsSafe(r,s,e2,t2) && GuardedEffectsInvariant(e2,effs2) by {
             Sound(e2,t2,effs);
           }
-          assert model.IsSafe(r,s,If(e,e1,e2),t') by { model.IteFalseSafe(r,s,e,e1,e2,t'); }
-          assert model.IsSafe(r,s,If(e,e1,e2),t) by {
-            model.SubtyCompat(t',t);
-            model.SemSubtyTransport(r,s,If(e,e1,e2),t',t);
+          assert IsSafe(r,s,If(e,e1,e2),t') by { IteFalseSafe(r,s,e,e1,e2,t'); }
+          assert IsSafe(r,s,If(e,e1,e2),t) by {
+            SubtyCompat(t',t);
+            SemSubtyTransport(r,s,If(e,e1,e2),t',t);
           }
           assert GuardedEffectsInvariant(If(e,e1,e2),effs2) by {
-            if model.IsTrueStrong(r,s,If(e,e1,e2)) {
-              model.IteTrueStrongFalse(r,s,e,e1,e2);
+            if IsTrueStrong(r,s,If(e,e1,e2)) {
+              IteTrueStrongFalse(r,s,e,e1,e2);
               assert EffectsInvariant(effs2);
             }
           }
@@ -257,65 +256,65 @@ module validation.thm.soundness {
           assert Typesafe(e2,effs,t2) by { SubtyRefl(t2); }
           assert t' == lubOpt(t1,t2).value;
           assert subty(t1,t') && subty(t2,t') by { LubIsUB(t1,t2,t'); }
-          if model.IsSafeStrong(r,s,e,Type.Bool(bt)) {
-            if model.IsTrue(r,s,e) {
+          if IsSafeStrong(r,s,e,Type.Bool(bt)) {
+            if IsTrue(r,s,e) {
               // `e` evaluates to true
-              model.IsTrueImpliesIsTrueStrong(r,s,e,Type.Bool(bt));
-              assert model.IsTrueStrong(r,s,e);
+              IsTrueImpliesIsTrueStrong(r,s,e,Type.Bool(bt));
+              assert IsTrueStrong(r,s,e);
               assert EffectsInvariant(effs1);
-              assert model.IsSafe(r,s,e1,t1) && GuardedEffectsInvariant(e1,effs2) by {
+              assert IsSafe(r,s,e1,t1) && GuardedEffectsInvariant(e1,effs2) by {
                 EffectsInvariantUnion(effs,effs1);
                 Sound(e1,t1,effs.union(effs1));
               }
-              assert model.IsSafe(r,s,If(e,e1,e2),t1) by { model.IteTrueSafe(r,s,e,e1,e2,t1); }
-              assert model.IsSafe(r,s,If(e,e1,e2),t) by {
-                model.SubtyCompat(t1,t');
-                model.SubtyCompat(t',t);
-                model.SemSubtyTransport(r,s,If(e,e1,e2),t1,t);
+              assert IsSafe(r,s,If(e,e1,e2),t1) by { IteTrueSafe(r,s,e,e1,e2,t1); }
+              assert IsSafe(r,s,If(e,e1,e2),t) by {
+                SubtyCompat(t1,t');
+                SubtyCompat(t',t);
+                SemSubtyTransport(r,s,If(e,e1,e2),t1,t);
               }
               assert GuardedEffectsInvariant(If(e,e1,e2),effs1.union(effs2)) by {
-                if model.IsTrueStrong(r,s,If(e,e1,e2)) {
-                  model.IteTrueStrongTrue(r,s,e,e1,e2);
+                if IsTrueStrong(r,s,If(e,e1,e2)) {
+                  IteTrueStrongTrue(r,s,e,e1,e2);
                   EffectsInvariantUnion(effs1,effs2);
                 }
               }
               assert GuardedEffectsInvariant(If(e,e1,e2),effs1.union(effs2).intersect(effs3)) by {
-                if model.IsTrueStrong(r,s,If(e,e1,e2)) {
+                if IsTrueStrong(r,s,If(e,e1,e2)) {
                   EffectsInvariantIntersectL(effs1.union(effs2),effs3);
                 }
               }
             } else {
               // `e` evaluates to false
-              model.NotTrueImpliesFalse(r,s,e,bt);
-              assert model.IsFalse(r,s,e);
-              assert model.IsSafe(r,s,e2,t2) && GuardedEffectsInvariant(e2,effs3) by {
+              NotTrueImpliesFalse(r,s,e,bt);
+              assert IsFalse(r,s,e);
+              assert IsSafe(r,s,e2,t2) && GuardedEffectsInvariant(e2,effs3) by {
                 Sound(e2,t2,effs);
               }
-              assert model.IsSafe(r,s,If(e,e1,e2),t2) by { model.IteFalseSafe(r,s,e,e1,e2,t2); }
-              assert model.IsSafe(r,s,If(e,e1,e2),t) by {
-                model.SubtyCompat(t2,t');
-                model.SubtyCompat(t',t);
-                model.SemSubtyTransport(r,s,If(e,e1,e2),t2,t);
+              assert IsSafe(r,s,If(e,e1,e2),t2) by { IteFalseSafe(r,s,e,e1,e2,t2); }
+              assert IsSafe(r,s,If(e,e1,e2),t) by {
+                SubtyCompat(t2,t');
+                SubtyCompat(t',t);
+                SemSubtyTransport(r,s,If(e,e1,e2),t2,t);
               }
               assert GuardedEffectsInvariant(If(e,e1,e2),effs3) by {
-                if model.IsTrueStrong(r,s,If(e,e1,e2)) {
-                  model.IteTrueStrongFalse(r,s,e,e1,e2);
+                if IsTrueStrong(r,s,If(e,e1,e2)) {
+                  IteTrueStrongFalse(r,s,e,e1,e2);
                 }
               }
               assert GuardedEffectsInvariant(If(e,e1,e2),effs1.union(effs2).intersect(effs3)) by {
-                if model.IsTrueStrong(r,s,If(e,e1,e2)) {
+                if IsTrueStrong(r,s,If(e,e1,e2)) {
                   EffectsInvariantIntersectR(effs1.union(effs2),effs3);
                 }
               }
             }
           } else {
             // `e` produces an error
-            assert model.IsSafe(r,s,If(e,e1,e2),t) by {
-              model.IteError(r,s,e,e1,e2,Type.Bool(bt),t);
+            assert IsSafe(r,s,If(e,e1,e2),t) by {
+              IteError(r,s,e,e1,e2,Type.Bool(bt),t);
             }
             assert GuardedEffectsInvariant(If(e,e1,e2),effs1.union(effs2).intersect(effs3)) by {
-              model.IteError(r,s,e,e1,e2,Type.Bool(bt),Type.Bool(True));
-              assert !model.IsTrueStrong(r,s,If(e,e1,e2));
+              IteError(r,s,e,e1,e2,Type.Bool(bt),Type.Bool(True));
+              assert !IsTrueStrong(r,s,If(e,e1,e2));
             }
           }
       }
@@ -328,14 +327,14 @@ module validation.thm.soundness {
       requires InstanceOfActionStore(s,acts)
       requires EffectsInvariant(effs)
       requires Typesafe(And(e1,e2),effs,t)
-      ensures model.IsSafe(r,s,And(e1,e2),t)
+      ensures IsSafe(r,s,And(e1,e2),t)
       ensures GuardedEffectsInvariant(And(e1,e2),getEffects(And(e1,e2),effs))
     {
       var t' :| getType(And(e1,e2),effs) == t' && subty(t',t);
       assert Typechecker(ets,acts,reqty).inferAnd(e1,e2,effs).Ok?;
       var (bt1, effs1) := Typechecker(ets,acts,reqty).inferBoolType(e1,effs).value;
       assert Typesafe(e1,effs,Type.Bool(bt1));
-      assert model.IsSafe(r,s,e1,Type.Bool(bt1)) && GuardedEffectsInvariant(e1,effs1) by {
+      assert IsSafe(r,s,e1,Type.Bool(bt1)) && GuardedEffectsInvariant(e1,effs1) by {
         Sound(e1,Type.Bool(bt1),effs);
       }
       assert GuardedEffectsInvariant(And(e1,e2),Effects.empty()) by {
@@ -343,78 +342,78 @@ module validation.thm.soundness {
       }
       match bt1 {
         case False =>
-          assert model.IsSafe(r,s,And(e1,e2),t') by { model.AndLShortSafe(r,s,e1,e2); }
-          assert model.IsSafe(r,s,And(e1,e2),t) by {
-            model.SubtyCompat(t',t);
-            model.SemSubtyTransport(r,s,And(e1,e2),t',t);
+          assert IsSafe(r,s,And(e1,e2),t') by { AndLShortSafe(r,s,e1,e2); }
+          assert IsSafe(r,s,And(e1,e2),t) by {
+            SubtyCompat(t',t);
+            SemSubtyTransport(r,s,And(e1,e2),t',t);
           }
         case _ =>
           var res := Typechecker(ets,acts,reqty).inferBoolType(e2,effs.union(effs1)).value;
           var bt2 := res.0;
           var effs2 := res.1;
           assert Typesafe(e2,effs.union(effs1),Type.Bool(bt2));
-          if model.IsSafeStrong(r,s,e1,Type.Bool(bt1)) {
-            if model.IsTrue(r,s,e1) {
+          if IsSafeStrong(r,s,e1,Type.Bool(bt1)) {
+            if IsTrue(r,s,e1) {
               // `e1` evaluates to true
-              model.IsTrueImpliesIsTrueStrong(r,s,e1,Type.Bool(bt1));
-              assert model.IsTrueStrong(r,s,e1);
+              IsTrueImpliesIsTrueStrong(r,s,e1,Type.Bool(bt1));
+              assert IsTrueStrong(r,s,e1);
               assert EffectsInvariant(effs1);
-              assert model.IsSafe(r,s,e2,Type.Bool(bt2)) && GuardedEffectsInvariant(e2,effs2) by {
+              assert IsSafe(r,s,e2,Type.Bool(bt2)) && GuardedEffectsInvariant(e2,effs2) by {
                 EffectsInvariantUnion(effs,effs1);
                 Sound(e2,Type.Bool(bt2),effs.union(effs1));
               }
               match bt2 {
                 case False =>
-                  assert model.IsFalse(r,s,e2);
-                  assert model.IsSafe(r,s,e1,Type.Bool(AnyBool)) by {
+                  assert IsFalse(r,s,e2);
+                  assert IsSafe(r,s,e1,Type.Bool(AnyBool)) by {
                     assert subty(Type.Bool(bt1),Type.Bool(AnyBool));
-                    model.SubtyCompat(Type.Bool(bt1),Type.Bool(AnyBool));
-                    model.SemSubtyTransport(r,s,e1,Type.Bool(bt1),Type.Bool(AnyBool));
+                    SubtyCompat(Type.Bool(bt1),Type.Bool(AnyBool));
+                    SemSubtyTransport(r,s,e1,Type.Bool(bt1),Type.Bool(AnyBool));
                   }
-                  assert model.IsSafe(r,s,And(e1,e2),t') by {
-                    model.AndRShortSafe(r,s,e1,e2);
+                  assert IsSafe(r,s,And(e1,e2),t') by {
+                    AndRShortSafe(r,s,e1,e2);
                   }
-                  assert model.IsSafe(r,s,And(e1,e2),t) by {
-                    model.SubtyCompat(t',t);
-                    model.SemSubtyTransport(r,s,And(e1,e2),t',t);
+                  assert IsSafe(r,s,And(e1,e2),t) by {
+                    SubtyCompat(t',t);
+                    SemSubtyTransport(r,s,And(e1,e2),t',t);
                   }
                 case True =>
-                  assert model.IsTrue(r,s,e2);
-                  assert model.SemanticSubty(Type.Bool(bt1),Type.Bool(AnyBool)) by {
+                  assert IsTrue(r,s,e2);
+                  assert SemanticSubty(Type.Bool(bt1),Type.Bool(AnyBool)) by {
                     assert subty(Type.Bool(bt1),Type.Bool(AnyBool));
-                    model.SubtyCompat(Type.Bool(bt1),Type.Bool(AnyBool));
+                    SubtyCompat(Type.Bool(bt1),Type.Bool(AnyBool));
                   }
-                  assert model.IsSafe(r,s,And(e1,e2),Type.Bool(bt1)) by {
-                    model.AndLRetSafe(r,s,e1,e2,Type.Bool(bt1));
+                  assert IsSafe(r,s,And(e1,e2),Type.Bool(bt1)) by {
+                    AndLRetSafe(r,s,e1,e2,Type.Bool(bt1));
                   }
-                  assert model.IsSafe(r,s,And(e1,e2),t) by {
-                    model.SubtyCompat(t',t);
-                    model.SemSubtyTransport(r,s,And(e1,e2),t',t);
+                  assert IsSafe(r,s,And(e1,e2),t) by {
+                    SubtyCompat(t',t);
+                    SemSubtyTransport(r,s,And(e1,e2),t',t);
                   }
                   assert GuardedEffectsInvariant(And(e1,e2),effs1.union(effs2)) by {
-                    if model.IsTrueStrong(r,s,And(e1,e2)) {
-                      model.AndTrueStrong(r,s,e1,e2);
+                    if IsTrueStrong(r,s,And(e1,e2)) {
+                      AndTrueStrong(r,s,e1,e2);
                       assert EffectsInvariant(effs2);
                       EffectsInvariantUnion(effs1,effs2);
                     }
                   }
                 case _ =>
-                  assert model.IsSafe(r,s,e1,Type.Bool(AnyBool)) by {
-                    model.SubtyCompat(Type.Bool(bt1),Type.Bool(AnyBool));
-                    model.SemSubtyTransport(r,s,e1,Type.Bool(bt1),Type.Bool(AnyBool));
+                  assert IsSafe(r,s,e1,Type.Bool(AnyBool)) by {
+                    SubtyCompat(Type.Bool(bt1),Type.Bool(AnyBool));
+                    SemSubtyTransport(r,s,e1,Type.Bool(bt1),Type.Bool(AnyBool));
                   }
-                  assert model.IsSafe(r,s,e2,Type.Bool(AnyBool)) by {
-                    model.SubtyCompat(Type.Bool(bt2),Type.Bool(AnyBool));
-                    model.SemSubtyTransport(r,s,e2,Type.Bool(bt2),Type.Bool(AnyBool));
+                  assert IsSafe(r,s,e2,Type.Bool(AnyBool)) by {
+                    SubtyCompat(Type.Bool(bt2),Type.Bool(AnyBool));
+                    SemSubtyTransport(r,s,e2,Type.Bool(bt2),Type.Bool(AnyBool));
                   }
-                  assert model.IsSafe(r,s,And(e1,e2),Type.Bool(AnyBool)) by { model.AndSafe(r,s,e1,e2); }
-                  assert model.IsSafe(r,s,And(e1,e2),t) by {
-                    model.SubtyCompat(t',t);
-                    model.SemSubtyTransport(r,s,And(e1,e2),t',t);
+                  assert IsSafe(r,s,And(e1,e2),Type.Bool(AnyBool)) by { AndSafe(r,s,e1,e2); }
+                  assert IsSafe(r,s,And(e1,e2),t) by {
+                    SubtyCompat(t',t);
+                    SemSubtyTransport(r,s,And(e1,e2),t',t);
                   }
                   assert GuardedEffectsInvariant(And(e1,e2),effs1.union(effs2)) by {
-                    if model.IsTrueStrong(r,s,And(e1,e2)) {
-                      model.AndTrueStrong(r,s,e1,e2);
+                    if IsTrueStrong(r,s,And(e1,e2)) {
+                      AndTrueStrong(r,s,e1,e2);
                       assert EffectsInvariant(effs2);
                       EffectsInvariantUnion(effs1,effs2);
                     }
@@ -422,37 +421,37 @@ module validation.thm.soundness {
               }
             } else {
               // `e1` evaluates to false
-              model.NotTrueImpliesFalse(r,s,e1,bt1);
-              assert model.IsFalse(r,s,e1);
-              assert model.IsFalse(r,s,And(e1,e2)) by { model.AndLShortSafe(r,s,e1,e2); }
-              assert model.IsSafe(r,s,And(e1,e2),t) by {
-                model.SubtyCompat(Type.Bool(False),t);
-                model.SemSubtyTransport(r,s,And(e1,e2),Type.Bool(False),t);
+              NotTrueImpliesFalse(r,s,e1,bt1);
+              assert IsFalse(r,s,e1);
+              assert IsFalse(r,s,And(e1,e2)) by { AndLShortSafe(r,s,e1,e2); }
+              assert IsSafe(r,s,And(e1,e2),t) by {
+                SubtyCompat(Type.Bool(False),t);
+                SemSubtyTransport(r,s,And(e1,e2),Type.Bool(False),t);
               }
               match bt2 {
                 case False =>
                 case True =>
                   assert GuardedEffectsInvariant(And(e1,e2),effs1.union(effs2)) by {
-                    assert model.IsFalse(r,s,And(e1,e2));
-                    model.FalseImpliesNotTrueStrong(r,s,And(e1,e2));
-                    assert !model.IsTrueStrong(r,s,And(e1,e2));
+                    assert IsFalse(r,s,And(e1,e2));
+                    FalseImpliesNotTrueStrong(r,s,And(e1,e2));
+                    assert !IsTrueStrong(r,s,And(e1,e2));
                   }
                 case AnyBool =>
                   assert GuardedEffectsInvariant(And(e1,e2),effs1.union(effs2)) by {
-                    assert model.IsFalse(r,s,And(e1,e2));
-                    model.FalseImpliesNotTrueStrong(r,s,And(e1,e2));
-                    assert !model.IsTrueStrong(r,s,And(e1,e2));
+                    assert IsFalse(r,s,And(e1,e2));
+                    FalseImpliesNotTrueStrong(r,s,And(e1,e2));
+                    assert !IsTrueStrong(r,s,And(e1,e2));
                   }
               }
             }
           } else {
             // `e1` produces an error
-            assert model.IsSafe(r,s,And(e1,e2),t) by {
-              model.AndError(r,s,e1,e2,Type.Bool(bt1),t);
+            assert IsSafe(r,s,And(e1,e2),t) by {
+              AndError(r,s,e1,e2,Type.Bool(bt1),t);
             }
             assert GuardedEffectsInvariant(And(e1,e2),effs1.union(effs2)) by {
-              model.AndError(r,s,e1,e2,Type.Bool(bt1),Type.Bool(True));
-              assert !model.IsTrueStrong(r,s,And(e1,e2));
+              AndError(r,s,e1,e2,Type.Bool(bt1),Type.Bool(True));
+              assert !IsTrueStrong(r,s,And(e1,e2));
             }
           }
       }
@@ -465,14 +464,14 @@ module validation.thm.soundness {
       requires InstanceOfActionStore(s,acts)
       requires EffectsInvariant(effs)
       requires Typesafe(Or(e1,e2),effs,t)
-      ensures model.IsSafe(r,s,Or(e1,e2),t)
+      ensures IsSafe(r,s,Or(e1,e2),t)
       ensures GuardedEffectsInvariant(Or(e1,e2),getEffects(Or(e1,e2),effs))
     {
       var t' :| getType(Or(e1,e2),effs) == t' && subty(t',t);
       assert Typechecker(ets,acts,reqty).inferOr(e1,e2,effs).Ok?;
       var (bt1, effs1) := Typechecker(ets,acts,reqty).inferBoolType(e1,effs).value;
       assert Typesafe(e1,effs,Type.Bool(bt1));
-      assert model.IsSafe(r,s,e1,Type.Bool(bt1)) && GuardedEffectsInvariant(e1,effs1) by {
+      assert IsSafe(r,s,e1,Type.Bool(bt1)) && GuardedEffectsInvariant(e1,effs1) by {
         Sound(e1,Type.Bool(bt1),effs);
       }
       assert GuardedEffectsInvariant(Or(e1,e2),Effects.empty()) by {
@@ -480,91 +479,91 @@ module validation.thm.soundness {
       }
       match bt1 {
         case True =>
-          assert model.IsTrue(r,s,e1);
-          assert model.IsSafe(r,s,Or(e1,e2),t') by { model.OrLShortSafe(r,s,e1,e2); }
-          assert model.IsSafe(r,s,Or(e1,e2),t) by {
-            model.SubtyCompat(t',t);
-            model.SemSubtyTransport(r,s,Or(e1,e2),t',t);
+          assert IsTrue(r,s,e1);
+          assert IsSafe(r,s,Or(e1,e2),t') by { OrLShortSafe(r,s,e1,e2); }
+          assert IsSafe(r,s,Or(e1,e2),t) by {
+            SubtyCompat(t',t);
+            SemSubtyTransport(r,s,Or(e1,e2),t',t);
           }
         case False =>
-          assert model.IsFalse(r,s,e1);
+          assert IsFalse(r,s,e1);
           var (bt2, effs2) := Typechecker(ets,acts,reqty).inferBoolType(e2,effs).value;
           assert Typesafe(e2,effs,Type.Bool(bt2));
-          assert model.IsSafe(r,s,e2,Type.Bool(bt2)) && GuardedEffectsInvariant(e2,effs2) by {
+          assert IsSafe(r,s,e2,Type.Bool(bt2)) && GuardedEffectsInvariant(e2,effs2) by {
             Sound(e2,Type.Bool(bt2),effs);
           }
-          assert model.SemanticSubty(Type.Bool(bt2),Type.Bool(AnyBool)) by {
+          assert SemanticSubty(Type.Bool(bt2),Type.Bool(AnyBool)) by {
             assert subty(Type.Bool(bt2),Type.Bool(AnyBool));
-            model.SubtyCompat(Type.Bool(bt2),Type.Bool(AnyBool));
+            SubtyCompat(Type.Bool(bt2),Type.Bool(AnyBool));
           }
-          assert model.IsSafe(r,s,Or(e1,e2),Type.Bool(bt2)) by { model.OrRRetSafe(r,s,e1,e2,Type.Bool(bt2)); }
-          assert model.IsSafe(r,s,Or(e1,e2),t) by {
-            model.SubtyCompat(t',t);
-            model.SemSubtyTransport(r,s,Or(e1,e2),t',t);
+          assert IsSafe(r,s,Or(e1,e2),Type.Bool(bt2)) by { OrRRetSafe(r,s,e1,e2,Type.Bool(bt2)); }
+          assert IsSafe(r,s,Or(e1,e2),t) by {
+            SubtyCompat(t',t);
+            SemSubtyTransport(r,s,Or(e1,e2),t',t);
           }
           assert GuardedEffectsInvariant(Or(e1,e2),effs2) by {
-            if model.IsTrueStrong(r,s,Or(e1,e2)) {
-              model.OrTrueStrong(r,s,e1,e2);
-              model.FalseImpliesNotTrueStrong(r,s,e1);
-              assert model.IsTrueStrong(r,s,e2);
+            if IsTrueStrong(r,s,Or(e1,e2)) {
+              OrTrueStrong(r,s,e1,e2);
+              FalseImpliesNotTrueStrong(r,s,e1);
+              assert IsTrueStrong(r,s,e2);
               assert EffectsInvariant(effs2);
             }
           }
         case _ =>
           var (bt2, effs2) := Typechecker(ets,acts,reqty).inferBoolType(e2,effs).value;
           assert Typesafe(e2,effs,Type.Bool(bt2));
-          assert model.IsSafe(r,s,e2,Type.Bool(bt2)) && GuardedEffectsInvariant(e2,effs2) by {
+          assert IsSafe(r,s,e2,Type.Bool(bt2)) && GuardedEffectsInvariant(e2,effs2) by {
             Sound(e2,Type.Bool(bt2),effs);
           }
           match bt2 {
             case True =>
-              assert model.IsTrue(r,s,e2);
-              assert model.IsSafe(r,s,e1,Type.Bool(AnyBool)) by {
-                model.SubtyCompat(Type.Bool(bt1),Type.Bool(AnyBool));
-                model.SemSubtyTransport(r,s,e1,Type.Bool(bt1),Type.Bool(AnyBool));
+              assert IsTrue(r,s,e2);
+              assert IsSafe(r,s,e1,Type.Bool(AnyBool)) by {
+                SubtyCompat(Type.Bool(bt1),Type.Bool(AnyBool));
+                SemSubtyTransport(r,s,e1,Type.Bool(bt1),Type.Bool(AnyBool));
               }
-              assert model.IsTrue(r,s,Or(e1,e2)) by { model.OrRShortSafe(r,s,e1,e2); }
-              assert model.IsSafe(r,s,Or(e1,e2),t) by {
-                model.SubtyCompat(Type.Bool(True),t);
-                model.SemSubtyTransport(r,s,Or(e1,e2),Type.Bool(True),t);
+              assert IsTrue(r,s,Or(e1,e2)) by { OrRShortSafe(r,s,e1,e2); }
+              assert IsSafe(r,s,Or(e1,e2),t) by {
+                SubtyCompat(Type.Bool(True),t);
+                SemSubtyTransport(r,s,Or(e1,e2),Type.Bool(True),t);
               }
             case False =>
-              assert model.IsFalse(r,s,e2);
-              assert model.IsSafe(r,s,Or(e1,e2),t) by {
-                model.OrLRetSafe(r,s,e1,e2,Type.Bool(bt1));
-                model.SubtyCompat(Type.Bool(bt1),t);
-                model.SemSubtyTransport(r,s,Or(e1,e2),Type.Bool(bt1),t);
+              assert IsFalse(r,s,e2);
+              assert IsSafe(r,s,Or(e1,e2),t) by {
+                OrLRetSafe(r,s,e1,e2,Type.Bool(bt1));
+                SubtyCompat(Type.Bool(bt1),t);
+                SemSubtyTransport(r,s,Or(e1,e2),Type.Bool(bt1),t);
               }
               assert GuardedEffectsInvariant(Or(e1,e2),effs1) by {
-                if model.IsTrueStrong(r,s,Or(e1,e2)) {
-                  model.OrTrueStrong(r,s,e1,e2);
-                  model.FalseImpliesNotTrueStrong(r,s,e2);
-                  assert model.IsTrueStrong(r,s,e1);
+                if IsTrueStrong(r,s,Or(e1,e2)) {
+                  OrTrueStrong(r,s,e1,e2);
+                  FalseImpliesNotTrueStrong(r,s,e2);
+                  assert IsTrueStrong(r,s,e1);
                   assert EffectsInvariant(effs1);
                 }
               }
             case _ =>
-              assert model.IsSafe(r,s,e1,Type.Bool(AnyBool)) by {
-                model.SubtyCompat(Type.Bool(bt1),Type.Bool(AnyBool));
-                model.SemSubtyTransport(r,s,e1,Type.Bool(bt1),Type.Bool(AnyBool));
+              assert IsSafe(r,s,e1,Type.Bool(AnyBool)) by {
+                SubtyCompat(Type.Bool(bt1),Type.Bool(AnyBool));
+                SemSubtyTransport(r,s,e1,Type.Bool(bt1),Type.Bool(AnyBool));
               }
-              assert model.IsSafe(r,s,e2,Type.Bool(AnyBool)) by {
-                model.SubtyCompat(Type.Bool(bt2),Type.Bool(AnyBool));
-                model.SemSubtyTransport(r,s,e2,Type.Bool(bt2),Type.Bool(AnyBool));
+              assert IsSafe(r,s,e2,Type.Bool(AnyBool)) by {
+                SubtyCompat(Type.Bool(bt2),Type.Bool(AnyBool));
+                SemSubtyTransport(r,s,e2,Type.Bool(bt2),Type.Bool(AnyBool));
               }
-              assert model.IsSafe(r,s,Or(e1,e2),Type.Bool(AnyBool)) by { model.OrSafe(r,s,e1,e2); }
-              assert model.IsSafe(r,s,Or(e1,e2),t) by {
-                model.SubtyCompat(t',t);
-                model.SemSubtyTransport(r,s,Or(e1,e2),t',t);
+              assert IsSafe(r,s,Or(e1,e2),Type.Bool(AnyBool)) by { OrSafe(r,s,e1,e2); }
+              assert IsSafe(r,s,Or(e1,e2),t) by {
+                SubtyCompat(t',t);
+                SemSubtyTransport(r,s,Or(e1,e2),t',t);
               }
               assert GuardedEffectsInvariant(Or(e1,e2),effs1.intersect(effs2)) by {
-                if model.IsTrueStrong(r,s,Or(e1,e2)) {
-                  model.OrTrueStrong(r,s,e1,e2);
-                  if model.IsTrueStrong(r,s,e1) {
+                if IsTrueStrong(r,s,Or(e1,e2)) {
+                  OrTrueStrong(r,s,e1,e2);
+                  if IsTrueStrong(r,s,e1) {
                     assert EffectsInvariant(effs1);
                     EffectsInvariantIntersectL(effs1,effs2);
                   } else {
-                    assert model.IsTrueStrong(r,s,e2);
+                    assert IsTrueStrong(r,s,e2);
                     assert EffectsInvariant(effs2);
                     EffectsInvariantIntersectR(effs1,effs2);
                   }
@@ -581,7 +580,7 @@ module validation.thm.soundness {
       requires InstanceOfActionStore(s,acts)
       requires EffectsInvariant(effs)
       requires Typesafe(UnaryApp(Not,e),effs,t)
-      ensures model.IsSafe(r,s,UnaryApp(Not,e),t)
+      ensures IsSafe(r,s,UnaryApp(Not,e),t)
       ensures getEffects(UnaryApp(Not,e),effs) == Effects.empty()
     {
       var t' :| getType(UnaryApp(Not,e),effs) == t' && subty(t',t);
@@ -589,17 +588,17 @@ module validation.thm.soundness {
       var (bt,_) := Typechecker(ets,acts,reqty).inferBoolType(e,effs).value;
       assert t' == Type.Bool(bt.not());
       assert Typesafe(e,effs,Type.Bool(bt)) by { SubtyRefl(Type.Bool(bt)); }
-      assert model.IsSafe(r,s,e,Type.Bool(bt)) by { Sound(e,Type.Bool(bt),effs); }
-      assert model.IsSafe(r,s,UnaryApp(Not,e),t') by {
+      assert IsSafe(r,s,e,Type.Bool(bt)) by { Sound(e,Type.Bool(bt),effs); }
+      assert IsSafe(r,s,UnaryApp(Not,e),t') by {
         match bt {
-          case AnyBool => model.NotSafe(r,s,e);
-          case True => model.NotTrueSafe(r,s,e);
-          case False => model.NotFalseSafe(r,s,e);
+          case AnyBool => NotSafe(r,s,e);
+          case True => NotTrueSafe(r,s,e);
+          case False => NotFalseSafe(r,s,e);
         }
       }
-      assert model.IsSafe(r,s,UnaryApp(Not,e),t) by {
-        model.SubtyCompat(t',t);
-        model.SemSubtyTransport(r,s,UnaryApp(Not,e),t',t);
+      assert IsSafe(r,s,UnaryApp(Not,e),t) by {
+        SubtyCompat(t',t);
+        SemSubtyTransport(r,s,UnaryApp(Not,e),t',t);
       }
     }
 
@@ -610,18 +609,18 @@ module validation.thm.soundness {
       requires InstanceOfActionStore(s,acts)
       requires EffectsInvariant(effs)
       requires Typesafe(UnaryApp(Neg,e),effs,t)
-      ensures model.IsSafe(r,s,UnaryApp(Neg,e),t)
+      ensures IsSafe(r,s,UnaryApp(Neg,e),t)
       ensures getEffects(UnaryApp(Neg,e),effs) == Effects.empty()
     {
       var t' :| getType(UnaryApp(Neg,e),effs) == t' && subty(t',t);
       assert Typechecker(ets,acts,reqty).inferArith1(Neg,e,effs) == types.Ok(Type.Int);
       assert Typechecker(ets,acts,reqty).ensureIntType(e,effs).Ok?;
       assert Typesafe(e,effs,Type.Int);
-      assert model.IsSafe(r,s,e,Type.Int) by { Sound(e,Type.Int,effs); }
-      assert model.IsSafe(r,s,UnaryApp(Neg,e),t') by { model.NegSafe(r,s,e); }
-      assert model.IsSafe(r,s,UnaryApp(Neg,e),t) by {
-        model.SubtyCompat(t',t);
-        model.SemSubtyTransport(r,s,UnaryApp(Neg,e),t',t);
+      assert IsSafe(r,s,e,Type.Int) by { Sound(e,Type.Int,effs); }
+      assert IsSafe(r,s,UnaryApp(Neg,e),t') by { NegSafe(r,s,e); }
+      assert IsSafe(r,s,UnaryApp(Neg,e),t) by {
+        SubtyCompat(t',t);
+        SemSubtyTransport(r,s,UnaryApp(Neg,e),t',t);
       }
     }
 
@@ -632,18 +631,18 @@ module validation.thm.soundness {
       requires InstanceOfActionStore(s,acts)
       requires EffectsInvariant(effs)
       requires Typesafe(UnaryApp(MulBy(i),e),effs,t)
-      ensures model.IsSafe(r,s,UnaryApp(MulBy(i),e),t)
+      ensures IsSafe(r,s,UnaryApp(MulBy(i),e),t)
       ensures getEffects(UnaryApp(MulBy(i),e),effs) == Effects.empty()
     {
       var t' :| getType(UnaryApp(MulBy(i),e),effs) == t' && subty(t',t);
       assert Typechecker(ets,acts,reqty).inferArith1(MulBy(i),e,effs) == types.Ok(Type.Int);
       assert Typechecker(ets,acts,reqty).ensureIntType(e,effs).Ok?;
       assert Typesafe(e,effs,Type.Int);
-      assert model.IsSafe(r,s,e,Type.Int) by { Sound(e,Type.Int,effs); }
-      assert model.IsSafe(r,s,UnaryApp(MulBy(i),e),t') by { model.MulBySafe(r,s,e,i); }
-      assert model.IsSafe(r,s,UnaryApp(MulBy(i),e),t) by {
-        model.SubtyCompat(t',t);
-        model.SemSubtyTransport(r,s,UnaryApp(MulBy(i),e),t',t);
+      assert IsSafe(r,s,e,Type.Int) by { Sound(e,Type.Int,effs); }
+      assert IsSafe(r,s,UnaryApp(MulBy(i),e),t') by { MulBySafe(r,s,e,i); }
+      assert IsSafe(r,s,UnaryApp(MulBy(i),e),t) by {
+        SubtyCompat(t',t);
+        SemSubtyTransport(r,s,UnaryApp(MulBy(i),e),t',t);
       }
     }
 
@@ -654,18 +653,18 @@ module validation.thm.soundness {
       requires InstanceOfActionStore(s,acts)
       requires EffectsInvariant(effs)
       requires Typesafe(UnaryApp(Like(p),e),effs,t)
-      ensures model.IsSafe(r,s,UnaryApp(Like(p),e),t)
+      ensures IsSafe(r,s,UnaryApp(Like(p),e),t)
       ensures getEffects(UnaryApp(Like(p),e),effs) == Effects.empty()
     {
       var t' :| getType(UnaryApp(Like(p),e),effs) == t' && subty(t',t);
       assert Typechecker(ets,acts,reqty).inferLike(p,e,effs) == types.Ok(Type.Bool(AnyBool));
       assert Typechecker(ets,acts,reqty).ensureStringType(e,effs).Ok?;
       assert Typesafe(e,effs,Type.String);
-      assert model.IsSafe(r,s,e,Type.String) by { Sound(e,Type.String,effs); }
-      assert model.IsSafe(r,s,UnaryApp(Like(p),e),t') by { model.LikeSafe(r,s,e,p); }
-      assert model.IsSafe(r,s,UnaryApp(Like(p),e),t) by {
-        model.SubtyCompat(t',t);
-        model.SemSubtyTransport(r,s,UnaryApp(Like(p),e),t',t);
+      assert IsSafe(r,s,e,Type.String) by { Sound(e,Type.String,effs); }
+      assert IsSafe(r,s,UnaryApp(Like(p),e),t') by { LikeSafe(r,s,e,p); }
+      assert IsSafe(r,s,UnaryApp(Like(p),e),t) by {
+        SubtyCompat(t',t);
+        SemSubtyTransport(r,s,UnaryApp(Like(p),e),t',t);
       }
     }
 
@@ -679,21 +678,21 @@ module validation.thm.soundness {
     lemma UnspecifiedVarHasUnspecifiedEntityType(e: Expr)
       requires Typechecker(ets,acts,reqty).isUnspecifiedVar(e)
       requires InstanceOfRequestType(r,reqty)
-      ensures model.IsSafe(r,s,e,unspecifiedEntityType)
+      ensures IsSafe(r,s,e,unspecifiedEntityType)
     {
       match e {
         case Var(Principal) =>
           assert r.principal == unspecifiedPrincipalEuid;
-          model.PrincipalIsSafe(r,s,unspecifiedEntityType);
+          PrincipalIsSafe(r,s,unspecifiedEntityType);
         case Var(Resource) =>
           assert r.resource == unspecifiedResourceEuid;
-          model.ResourceIsSafe(r,s,unspecifiedEntityType);
+          ResourceIsSafe(r,s,unspecifiedEntityType);
       }
     }
 
     lemma SoundEqAux(u1: EntityUID, u2: EntityUID, t: Type, effs: Effects)
       requires Typesafe(BinaryApp(BinaryOp.Eq,PrimitiveLit(Primitive.EntityUID(u1)),PrimitiveLit(Primitive.EntityUID(u2))),effs,t)
-      ensures model.IsSafe(r,s,BinaryApp(BinaryOp.Eq,PrimitiveLit(Primitive.EntityUID(u1)),PrimitiveLit(Primitive.EntityUID(u2))),t)
+      ensures IsSafe(r,s,BinaryApp(BinaryOp.Eq,PrimitiveLit(Primitive.EntityUID(u1)),PrimitiveLit(Primitive.EntityUID(u2))),t)
     {
       var e1: Expr := PrimitiveLit(Primitive.EntityUID(u1));
       var e2: Expr := PrimitiveLit(Primitive.EntityUID(u2));
@@ -704,16 +703,16 @@ module validation.thm.soundness {
       var t2 := getType(e2,effs);
       if u1 == u2 {
         assert t' == Type.Bool(True);
-        assert model.IsSafe(r,s,BinaryApp(BinaryOp.Eq,e1,e2),t') by { model.EqEntitySameSafe(r,s,u1); }
-        assert model.IsSafe(r,s,BinaryApp(BinaryOp.Eq,e1,e2),t) by {
-          model.SubtyCompat(t',t);
-          model.SemSubtyTransport(r,s,BinaryApp(BinaryOp.Eq,e1,e2),t',t); }
+        assert IsSafe(r,s,BinaryApp(BinaryOp.Eq,e1,e2),t') by { EqEntitySameSafe(r,s,u1); }
+        assert IsSafe(r,s,BinaryApp(BinaryOp.Eq,e1,e2),t) by {
+          SubtyCompat(t',t);
+          SemSubtyTransport(r,s,BinaryApp(BinaryOp.Eq,e1,e2),t',t); }
       } else {
         assert t' == Type.Bool(False);
-        assert model.IsSafe(r,s,BinaryApp(BinaryOp.Eq,e1,e2),t') by { model.EqEntityDiffSafe(r,s,u1,u2); }
-        assert model.IsSafe(r,s,BinaryApp(BinaryOp.Eq,e1,e2),t) by {
-          model.SubtyCompat(t',t);
-          model.SemSubtyTransport(r,s,BinaryApp(BinaryOp.Eq,e1,e2),t',t); }
+        assert IsSafe(r,s,BinaryApp(BinaryOp.Eq,e1,e2),t') by { EqEntityDiffSafe(r,s,u1,u2); }
+        assert IsSafe(r,s,BinaryApp(BinaryOp.Eq,e1,e2),t) by {
+          SubtyCompat(t',t);
+          SemSubtyTransport(r,s,BinaryApp(BinaryOp.Eq,e1,e2),t',t); }
       }
     }
 
@@ -724,7 +723,7 @@ module validation.thm.soundness {
       requires InstanceOfActionStore(s,acts)
       requires EffectsInvariant(effs)
       requires Typesafe(BinaryApp(BinaryOp.Eq,e1,e2),effs,t)
-      ensures model.IsSafe(r,s,BinaryApp(BinaryOp.Eq,e1,e2),t)
+      ensures IsSafe(r,s,BinaryApp(BinaryOp.Eq,e1,e2),t)
       ensures getEffects(BinaryApp(BinaryOp.Eq,e1,e2),effs) == Effects.empty()
     {
       var t' :| getType(BinaryApp(BinaryOp.Eq,e1,e2),effs) == t' && subty(t',t);
@@ -733,26 +732,26 @@ module validation.thm.soundness {
       var t2 := getType(e2,effs);
       assert Typesafe(e1,effs,t1) by { SubtyRefl(t1); }
       assert Typesafe(e2,effs,t2) by { SubtyRefl(t2); }
-      assert model.IsSafe(r,s,e1,t1) by { Sound(e1,t1,effs); }
-      assert model.IsSafe(r,s,e2,t2) by { Sound(e2,t2,effs); }
+      assert IsSafe(r,s,e1,t1) by { Sound(e1,t1,effs); }
+      assert IsSafe(r,s,e2,t2) by { Sound(e2,t2,effs); }
       match (e1,e2,t1,t2) {
         case (PrimitiveLit(EntityUID(u1)),PrimitiveLit(EntityUID(u2)),_,_) =>
           SoundEqAux(u1,u2,t,effs);
         case _ =>
           if t1.Entity? && t2.Entity? && t1.lub.disjoint(t2.lub) {
             assert t' == Type.Bool(False);
-            model.EqFalseIsSafe(r,s,e1,e2,t1.lub,t2.lub);
+            EqFalseIsSafe(r,s,e1,e2,t1.lub,t2.lub);
           } else if Typechecker(ets,acts,reqty).isUnspecifiedVar(e1) && t2.Entity? && t2.lub.specified() {
             assert t' == Type.Bool(False);
             UnspecifiedVarHasUnspecifiedEntityType(e1);
-            model.EqFalseIsSafe(r,s,e1,e2,unspecifiedEntityType.lub,t2.lub);
+            EqFalseIsSafe(r,s,e1,e2,unspecifiedEntityType.lub,t2.lub);
           } else {
             assert t' == Type.Bool(AnyBool);
-            model.EqIsSafe(r,s,e1,e2,t1,t2);
+            EqIsSafe(r,s,e1,e2,t1,t2);
           }
-          assert model.IsSafe(r,s,BinaryApp(BinaryOp.Eq,e1,e2),t) by {
-            model.SubtyCompat(t',t);
-            model.SemSubtyTransport(r,s,BinaryApp(BinaryOp.Eq,e1,e2),t',t);
+          assert IsSafe(r,s,BinaryApp(BinaryOp.Eq,e1,e2),t) by {
+            SubtyCompat(t',t);
+            SemSubtyTransport(r,s,BinaryApp(BinaryOp.Eq,e1,e2),t',t);
           }
       }
     }
@@ -765,7 +764,7 @@ module validation.thm.soundness {
       requires InstanceOfActionStore(s,acts)
       requires EffectsInvariant(effs)
       requires Typesafe(BinaryApp(op,e1,e2),effs,t)
-      ensures model.IsSafe(r,s,BinaryApp(op,e1,e2),t)
+      ensures IsSafe(r,s,BinaryApp(op,e1,e2),t)
       ensures getEffects(BinaryApp(op,e1,e2),effs) == Effects.empty()
     {
       var t' :| getType(BinaryApp(op,e1,e2),effs) == t' && subty(t',t);
@@ -774,12 +773,12 @@ module validation.thm.soundness {
       assert Typesafe(e1,effs,Type.Int);
       assert Typechecker(ets,acts,reqty).ensureIntType(e2,effs).Ok?;
       assert Typesafe(e2,effs,Type.Int);
-      assert model.IsSafe(r,s,e1,Type.Int) by { Sound(e1,Type.Int,effs); }
-      assert model.IsSafe(r,s,e2,Type.Int) by { Sound(e2,Type.Int,effs); }
-      assert model.IsSafe(r,s,BinaryApp(op,e1,e2),t') by { model.IneqSafe(r,s,op,e1,e2); }
-      assert model.IsSafe(r,s,BinaryApp(op,e1,e2),t) by {
-        model.SubtyCompat(t',t);
-        model.SemSubtyTransport(r,s,BinaryApp(op,e1,e2),t',t);
+      assert IsSafe(r,s,e1,Type.Int) by { Sound(e1,Type.Int,effs); }
+      assert IsSafe(r,s,e2,Type.Int) by { Sound(e2,Type.Int,effs); }
+      assert IsSafe(r,s,BinaryApp(op,e1,e2),t') by { IneqSafe(r,s,op,e1,e2); }
+      assert IsSafe(r,s,BinaryApp(op,e1,e2),t) by {
+        SubtyCompat(t',t);
+        SemSubtyTransport(r,s,BinaryApp(op,e1,e2),t',t);
       }
     }
 
@@ -791,7 +790,7 @@ module validation.thm.soundness {
       requires InstanceOfActionStore(s,acts)
       requires EffectsInvariant(effs)
       requires Typesafe(BinaryApp(op,e1,e2),effs,t)
-      ensures model.IsSafe(r,s,BinaryApp(op,e1,e2),t)
+      ensures IsSafe(r,s,BinaryApp(op,e1,e2),t)
       ensures getEffects(BinaryApp(op,e1,e2),effs) == Effects.empty()
     {
       var t' :| getType(BinaryApp(op,e1,e2),effs) == t' && subty(t',t);
@@ -800,12 +799,12 @@ module validation.thm.soundness {
       assert Typesafe(e1,effs,Type.Int);
       assert Typechecker(ets,acts,reqty).ensureIntType(e2,effs).Ok?;
       assert Typesafe(e2,effs,Type.Int);
-      assert model.IsSafe(r,s,e1,Type.Int) by { Sound(e1,Type.Int,effs); }
-      assert model.IsSafe(r,s,e2,Type.Int) by { Sound(e2,Type.Int,effs); }
-      assert model.IsSafe(r,s,BinaryApp(op,e1,e2),t') by { model.ArithSafe(r,s,op,e1,e2); }
-      assert model.IsSafe(r,s,BinaryApp(op,e1,e2),t) by {
-        model.SubtyCompat(t',t);
-        model.SemSubtyTransport(r,s,BinaryApp(op,e1,e2),t',t);
+      assert IsSafe(r,s,e1,Type.Int) by { Sound(e1,Type.Int,effs); }
+      assert IsSafe(r,s,e2,Type.Int) by { Sound(e2,Type.Int,effs); }
+      assert IsSafe(r,s,BinaryApp(op,e1,e2),t') by { ArithSafe(r,s,op,e1,e2); }
+      assert IsSafe(r,s,BinaryApp(op,e1,e2),t) by {
+        SubtyCompat(t',t);
+        SemSubtyTransport(r,s,BinaryApp(op,e1,e2),t',t);
       }
     }
 
@@ -817,7 +816,7 @@ module validation.thm.soundness {
       requires InstanceOfActionStore(s,acts)
       requires EffectsInvariant(effs)
       requires Typesafe(BinaryApp(op,e1,e2),effs,t)
-      ensures model.IsSafe(r,s,BinaryApp(op,e1,e2),t)
+      ensures IsSafe(r,s,BinaryApp(op,e1,e2),t)
       ensures getEffects(BinaryApp(op,e1,e2),effs) == Effects.empty()
     {
       var t' :| getType(BinaryApp(op,e1,e2),effs) == t' && subty(t',t);
@@ -826,12 +825,12 @@ module validation.thm.soundness {
       var t2 := Typechecker(ets,acts,reqty).inferSetType(e2,effs).value;
       assert Typesafe(e1,effs,Type.Set(t1)) by { SubtyRefl(Type.Set(t1)); }
       assert Typesafe(e2,effs,Type.Set(t2)) by { SubtyRefl(Type.Set(t2)); }
-      assert model.IsSafe(r,s,e1,Type.Set(t1)) by { Sound(e1,Type.Set(t1),effs); }
-      assert model.IsSafe(r,s,e2,Type.Set(t2)) by { Sound(e2,Type.Set(t2),effs); }
-      assert model.IsSafe(r,s,BinaryApp(op,e1,e2),t') by { model.ContainsAnyAllSafe(r,s,op,e1,e2,t1,t2); }
-      assert model.IsSafe(r,s,BinaryApp(op,e1,e2),t) by {
-        model.SubtyCompat(t',t);
-        model.SemSubtyTransport(r,s,BinaryApp(op,e1,e2),t',t);
+      assert IsSafe(r,s,e1,Type.Set(t1)) by { Sound(e1,Type.Set(t1),effs); }
+      assert IsSafe(r,s,e2,Type.Set(t2)) by { Sound(e2,Type.Set(t2),effs); }
+      assert IsSafe(r,s,BinaryApp(op,e1,e2),t') by { ContainsAnyAllSafe(r,s,op,e1,e2,t1,t2); }
+      assert IsSafe(r,s,BinaryApp(op,e1,e2),t) by {
+        SubtyCompat(t',t);
+        SemSubtyTransport(r,s,BinaryApp(op,e1,e2),t',t);
       }
     }
 
@@ -842,7 +841,7 @@ module validation.thm.soundness {
       requires InstanceOfActionStore(s,acts)
       requires EffectsInvariant(effs)
       requires Typesafe(BinaryApp(Contains,e1,e2),effs,t)
-      ensures model.IsSafe(r,s,BinaryApp(Contains,e1,e2),t)
+      ensures IsSafe(r,s,BinaryApp(Contains,e1,e2),t)
       ensures getEffects(BinaryApp(Contains,e1,e2),effs) == Effects.empty()
     {
       var t' :| getType(BinaryApp(Contains,e1,e2),effs) == t' && subty(t',t);
@@ -851,18 +850,18 @@ module validation.thm.soundness {
       assert Typesafe(e1,effs,Type.Set(t1)) by { SubtyRefl(Type.Set(t1)); }
       var (t2,_) := Typechecker(ets,acts,reqty).infer(e2,effs).value;
       assert Typesafe(e2,effs,t2) by { SubtyRefl(t2); }
-      assert model.IsSafe(r,s,e1,Type.Set(t1)) by { Sound(e1,Type.Set(t1),effs); }
-      assert model.IsSafe(r,s,e2,t2) by { Sound(e2,t2,effs); }
-      assert model.IsSafe(r,s,BinaryApp(Contains,e1,e2),t') by { model.ContainsSetSafe(r,s,e1,e2,t1,t2); }
-      assert model.IsSafe(r,s,BinaryApp(Contains,e1,e2),t) by { model.SemSubtyTransport(r,s,BinaryApp(Contains,e1,e2),t',t); }
+      assert IsSafe(r,s,e1,Type.Set(t1)) by { Sound(e1,Type.Set(t1),effs); }
+      assert IsSafe(r,s,e2,t2) by { Sound(e2,t2,effs); }
+      assert IsSafe(r,s,BinaryApp(Contains,e1,e2),t') by { ContainsSetSafe(r,s,e1,e2,t1,t2); }
+      assert IsSafe(r,s,BinaryApp(Contains,e1,e2),t) by { SemSubtyTransport(r,s,BinaryApp(Contains,e1,e2),t',t); }
     }
 
     lemma InferRecordLemma(e: Expr, es: seq<(Attr,Expr)>, effs: Effects)
-      requires forall i :: 0 <= i < |es| ==> es[i] < e
+      requires forall i | 0 <= i < |es| :: es[i] < e
       requires Typechecker(ets,acts,reqty).inferRecord(e,es,effs).Ok?
-      ensures forall i :: 0 <= i < |es| ==> es[i].0 in Typechecker(ets,acts,reqty).inferRecord(e,es,effs).value.Keys && Typechecker(ets,acts,reqty).infer(es[i].1,effs).Ok?
-      ensures forall k :: k in Typechecker(ets,acts,reqty).inferRecord(e,es,effs).value.Keys ==> KeyExists(k,es) && Typechecker(ets,acts,reqty).infer(LastOfKey(k,es),effs).value.0 == Typechecker(ets,acts,reqty).inferRecord(e,es,effs).value[k].ty
-      ensures forall k :: !(k in Typechecker(ets,acts,reqty).inferRecord(e,es,effs).value.Keys) ==> !KeyExists(k,es)
+      ensures forall i | 0 <= i < |es| :: es[i].0 in Typechecker(ets,acts,reqty).inferRecord(e,es,effs).value.Keys && Typechecker(ets,acts,reqty).infer(es[i].1,effs).Ok?
+      ensures forall k | k in Typechecker(ets,acts,reqty).inferRecord(e,es,effs).value.Keys :: KeyExists(k,es) && Typechecker(ets,acts,reqty).infer(LastOfKey(k,es),effs).value.0 == Typechecker(ets,acts,reqty).inferRecord(e,es,effs).value[k].ty
+      ensures forall k | !(k in Typechecker(ets,acts,reqty).inferRecord(e,es,effs).value.Keys) :: !KeyExists(k,es)
     {
       reveal Typechecker(ets,acts,reqty).inferRecord();
     }
@@ -874,7 +873,7 @@ module validation.thm.soundness {
       requires InstanceOfActionStore(s,acts)
       requires EffectsInvariant(effs)
       requires Typesafe(Expr.Record(es),effs,t)
-      ensures model.IsSafe(r,s,Expr.Record(es),t)
+      ensures IsSafe(r,s,Expr.Record(es),t)
       ensures getEffects(Expr.Record(es),effs) == Effects.empty()
     {
       var t' :| getType(Expr.Record(es),effs) == t' && subty(t',t);
@@ -882,44 +881,46 @@ module validation.thm.soundness {
       InferRecordLemma(Expr.Record(es),es,effs);
       assert t' == Type.Record(rt);
       assert forall i | 0 <= i < |es| :: WellTyped(es[i].1,effs);
-      forall ae | ae in es
-        ensures exists t_ae :: model.IsSafe(r,s,ae.1,t_ae)
-      {
-        assert WellTyped(ae.1,effs);
-        var t_ae := getType(ae.1,effs);
-        assert Typesafe(ae.1,effs,t_ae) by { SubtyRefl(t_ae); }
-        assert model.IsSafe(r,s,ae.1,t_ae) by { Sound(ae.1,t_ae,effs); }
-      }
       assert forall k | k in rt :: KeyExists(k,es) && getType(LastOfKey(k,es),effs) == rt[k].ty by {
         assert Typechecker(ets,acts,reqty).inferRecord(Expr.Record(es),es,effs).Ok?;
       }
       forall k | k in rt
-        ensures KeyExists(k,es) && model.IsSafe(r,s,LastOfKey(k,es),rt[k].ty)
+        ensures KeyExists(k,es) && IsSafe(r,s,LastOfKey(k,es),rt[k].ty)
       {
         assert getType(LastOfKey(k,es),effs) == rt[k].ty;
         assert Typesafe(LastOfKey(k,es),effs,rt[k].ty) by { SubtyRefl(rt[k].ty); }
-        assert model.IsSafe(r,s,LastOfKey(k,es),rt[k].ty) by { Sound(LastOfKey(k,es),rt[k].ty,effs); }
+        assert IsSafe(r,s,LastOfKey(k,es),rt[k].ty) by { Sound(LastOfKey(k,es),rt[k].ty,effs); }
       }
-      assert model.IsSafe(r,s,Expr.Record(es),t') by {
-        model.RecordSafe(r,s,es,rt);
+      assert IsSafe(r,s,Expr.Record(es),t') by {
+        assert forall ae | ae in es :: ExistsSafeType(r,s,ae.1) by {
+          forall ae | ae in es
+            ensures ExistsSafeType(r,s,ae.1)
+          {
+            assert WellTyped(ae.1,effs);
+            var t_ae := getType(ae.1,effs);
+            assert Typesafe(ae.1,effs,t_ae) by { SubtyRefl(t_ae); }
+            assert IsSafe(r,s,ae.1,t_ae) by { Sound(ae.1,t_ae,effs); }
+          }
+        }
+        RecordSafe(r,s,es,rt);
       }
-      assert model.IsSafe(r,s,Expr.Record(es),t) by {
-        model.SubtyCompat(t',t);
-        model.SemSubtyTransport(r,s,Expr.Record(es),t',t);
+      assert IsSafe(r,s,Expr.Record(es),t) by {
+        SubtyCompat(t',t);
+        SemSubtyTransport(r,s,Expr.Record(es),t',t);
       }
     }
 
     lemma InferSetLemma(e: Expr, es: seq<Expr>, effs: Effects)
-      requires forall i :: 0 <= i < |es| ==> es[i] < e
+      requires forall i | 0 <= i < |es| :: es[i] < e
       requires Typechecker(ets,acts,reqty).inferSet(e,es,effs).Ok?
-      ensures forall i :: 0 <= i < |es| ==> Typechecker(ets,acts,reqty).infer(es[i],effs).Ok? && subty(Typechecker(ets,acts,reqty).infer(es[i],effs).value.0,Typechecker(ets,acts,reqty).inferSet(e,es,effs).value)
+      ensures forall i | 0 <= i < |es| :: Typechecker(ets,acts,reqty).infer(es[i],effs).Ok? && subty(Typechecker(ets,acts,reqty).infer(es[i],effs).value.0,Typechecker(ets,acts,reqty).inferSet(e,es,effs).value)
     {
       if es == [] {
       } else {
         var (t,_) := Typechecker(ets,acts,reqty).infer(es[0],effs).value;
         var t1 := Typechecker(ets,acts,reqty).inferSet(e,es[1..],effs).value;
         var t2 := lubOpt(t,t1).value;
-        assert forall i :: 0 <= i < |es| ==> Typechecker(ets,acts,reqty).infer(es[i],effs).Ok? && subty(Typechecker(ets,acts,reqty).infer(es[i],effs).value.0,t2) by {
+        assert forall i | 0 <= i < |es| :: Typechecker(ets,acts,reqty).infer(es[i],effs).Ok? && subty(Typechecker(ets,acts,reqty).infer(es[i],effs).value.0,t2) by {
           forall i | 0 <= i < |es|
             ensures Typechecker(ets,acts,reqty).infer(es[i],effs).Ok? && subty(Typechecker(ets,acts,reqty).infer(es[i],effs).value.0,t2)
           {
@@ -944,7 +945,7 @@ module validation.thm.soundness {
       requires InstanceOfActionStore(s,acts)
       requires Typesafe(Expr.Set(es),effs,t)
       requires EffectsInvariant(effs)
-      ensures model.IsSafe(r,s,Expr.Set(es),t)
+      ensures IsSafe(r,s,Expr.Set(es),t)
       ensures getEffects(Expr.Set(es),effs) == Effects.empty()
     {
       var t' :| getType(Expr.Set(es),effs) == t' && subty(t',t);
@@ -952,18 +953,18 @@ module validation.thm.soundness {
       InferSetLemma(Expr.Set(es),es,effs);
       assert t' == Type.Set(st);
       forall i | 0 <= i < |es|
-        ensures model.IsSafe(r,s,es[i],st)
+        ensures IsSafe(r,s,es[i],st)
       {
         InterpretSetLemma(es,r,s);
         assert Typesafe(es[i],effs,st);
         Sound(es[i],st,effs);
       }
-      assert model.IsSafe(r,s,Expr.Set(es),t') by {
-        model.SetConstrSafe(r,s,es,st);
+      assert IsSafe(r,s,Expr.Set(es),t') by {
+        SetConstrSafe(r,s,es,st);
       }
-      assert model.IsSafe(r,s,Expr.Set(es),t) by {
-        model.SubtyCompat(t',t);
-        model.SemSubtyTransport(r,s,Expr.Set(es),t',t);
+      assert IsSafe(r,s,Expr.Set(es),t) by {
+        SubtyCompat(t',t);
+        SemSubtyTransport(r,s,Expr.Set(es),t',t);
       }
     }
 
@@ -974,7 +975,7 @@ module validation.thm.soundness {
       requires InstanceOfActionStore(s,acts)
       requires EffectsInvariant(effs)
       requires Typesafe(GetAttr(e,k),effs,t)
-      ensures model.IsSafe(r,s,GetAttr(e,k),t)
+      ensures IsSafe(r,s,GetAttr(e,k),t)
       ensures getEffects(GetAttr(e,k),effs) == Effects.empty()
     {
       var t' :| getType(GetAttr(e,k),effs) == t' && subty(t',t);
@@ -984,46 +985,46 @@ module validation.thm.soundness {
         case Record(rt) => {
           assert t' == rt[k].ty;
           assert Typesafe(e,effs,Type.Record(rt)) by { SubtyRefl(Type.Record(rt)); }
-          assert model.IsSafe(r,s,e,Type.Record(rt)) by { Sound(e,Type.Record(rt),effs); }
-          assert model.IsSafe(r,s,GetAttr(e,k),t') by {
+          assert IsSafe(r,s,e,Type.Record(rt)) by { Sound(e,Type.Record(rt),effs); }
+          assert IsSafe(r,s,GetAttr(e,k),t') by {
             assert k in rt;
             assert rt[k].isRequired || effs.contains(e,k);
             if rt[k].isRequired {
-              model.ObjectProjSafeRequired(r,s,e,Type.Record(rt),k,rt[k]);
+              ObjectProjSafeRequired(r,s,e,Type.Record(rt),k,rt[k]);
             } else {
               reveal EffectsInvariant();
-              assert model.GetAttrSafe(r,s,e,k);
-              model.ObjectProjSafeGetAttrSafe(r,s,e,Type.Record(rt),k,rt[k]);
+              assert GetAttrSafe(r,s,e,k);
+              ObjectProjSafeGetAttrSafe(r,s,e,Type.Record(rt),k,rt[k]);
             }
           }
-          assert model.IsSafe(r,s,GetAttr(e,k),t) by {
-            model.SubtyCompat(t',t);
-            model.SemSubtyTransport(r,s,GetAttr(e,k),t',t);
+          assert IsSafe(r,s,GetAttr(e,k),t) by {
+            SubtyCompat(t',t);
+            SemSubtyTransport(r,s,GetAttr(e,k),t',t);
           }
         }
         case Entity(lub) => {
           var rt := ets.getLubRecordType(lub).value;
           assert t' == rt[k].ty;
-          assert model.IsSafe(r,s,e,Type.Entity(lub)) by { Sound(e,Type.Entity(lub),effs); }
-          assert model.IsSafe(r,s,GetAttr(e,k),t') by {
+          assert IsSafe(r,s,e,Type.Entity(lub)) by { Sound(e,Type.Entity(lub),effs); }
+          assert IsSafe(r,s,GetAttr(e,k),t') by {
             assert k in rt;
             assert rt[k].isRequired || effs.contains(e,k);
             if !rt[k].isRequired {
               reveal EffectsInvariant();
-              assert model.GetAttrSafe(r,s,e,k);
+              assert GetAttrSafe(r,s,e,k);
             }
             forall euid: EntityUID | InstanceOfType(Primitive(Primitive.EntityUID(euid)),Type.Entity(lub)) && euid in s.entities
               ensures rt[k].isRequired ==> k in s.entities[euid].attrs
               ensures k in s.entities[euid].attrs ==> InstanceOfType(s.entities[euid].attrs[k],t')
             {
               GetLubRecordTypeSubty(lub, euid.ty);
-              model.SubtyCompat(ets.types[euid.ty][k].ty, t');
+              SubtyCompat(ets.types[euid.ty][k].ty, t');
             }
-            model.EntityProjSafe(r,s,e,k,lub,t',rt[k].isRequired);
+            EntityProjSafe(r,s,e,k,lub,t',rt[k].isRequired);
           }
-          assert model.IsSafe(r,s,GetAttr(e,k),t) by {
-            model.SubtyCompat(t',t);
-            model.SemSubtyTransport(r,s,GetAttr(e,k),t',t);
+          assert IsSafe(r,s,GetAttr(e,k),t) by {
+            SubtyCompat(t',t);
+            SemSubtyTransport(r,s,GetAttr(e,k),t',t);
           }
         }
       }
@@ -1040,6 +1041,7 @@ module validation.thm.soundness {
         var al := rtl[k];
         var a1 := rt1[k];
         var a2 := rt2[k];
+        assert lubOpt(a1.ty,a2.ty) == Ok(al.ty);
         LubIsUB(a1.ty, a2.ty, al.ty);
       }
     }
@@ -1085,7 +1087,7 @@ module validation.thm.soundness {
       requires InstanceOfActionStore(s,acts)
       requires EffectsInvariant(effs)
       requires Typesafe(HasAttr(e,k),effs,t)
-      ensures model.IsSafe(r,s,HasAttr(e,k),t)
+      ensures IsSafe(r,s,HasAttr(e,k),t)
       ensures GuardedEffectsInvariant(HasAttr(e,k),getEffects(HasAttr(e,k),effs))
     {
       var t' :| getType(HasAttr(e,k),effs) == t' && subty(t',t);
@@ -1097,82 +1099,82 @@ module validation.thm.soundness {
       match ret {
         case Record(rt) => {
           assert Typesafe(e,effs,Type.Record(rt)) by { SubtyRefl(Type.Record(rt)); }
-          assert model.IsSafe(r,s,e,Type.Record(rt)) by { Sound(e,Type.Record(rt),effs); }
+          assert IsSafe(r,s,e,Type.Record(rt)) by { Sound(e,Type.Record(rt),effs); }
           if k in rt {
             if rt[k].isRequired {
-              assert model.IsSafe(r,s,e,Type.Record(map[k := rt[k]])) by {
+              assert IsSafe(r,s,e,Type.Record(map[k := rt[k]])) by {
                 SubtyRefl(rt[k].ty);
                 assert subtyRecordType(rt,map[k := rt[k]]);
                 assert subty(Type.Record(rt),Type.Record(map[k := rt[k]]));
-                model.SubtyCompat(Type.Record(rt),Type.Record(map[k := rt[k]]));
-                model.SemSubtyTransport(r,s,e,Type.Record(rt),Type.Record(map[k := rt[k]]));
+                SubtyCompat(Type.Record(rt),Type.Record(map[k := rt[k]]));
+                SemSubtyTransport(r,s,e,Type.Record(rt),Type.Record(map[k := rt[k]]));
               }
-              assert model.IsSafe(r,s,HasAttr(e,k),t') by { model.RecordHasRequiredTrueSafe(r,s,e,k,rt[k]); }
+              assert IsSafe(r,s,HasAttr(e,k),t') by { RecordHasRequiredTrueSafe(r,s,e,k,rt[k]); }
             } else if effs.contains(e,k) {
-              assert model.IsSafe(r,s,HasAttr(e,k),t') by {
+              assert IsSafe(r,s,HasAttr(e,k),t') by {
                 reveal EffectsInvariant();
               }
             } else {
-              assert model.IsSafe(r,s,e,Type.Record(map[])) by {
+              assert IsSafe(r,s,e,Type.Record(map[])) by {
                 assert subty(Type.Record(rt),Type.Record(map[]));
-                model.SubtyCompat(Type.Record(rt),Type.Record(map[]));
-                model.SemSubtyTransport(r,s,e,Type.Record(rt),Type.Record(map[]));
+                SubtyCompat(Type.Record(rt),Type.Record(map[]));
+                SemSubtyTransport(r,s,e,Type.Record(rt),Type.Record(map[]));
               }
-              assert model.IsSafe(r,s,HasAttr(e,k),t') by { model.RecordHasOpenRecSafe(r,s,e,k); }
+              assert IsSafe(r,s,HasAttr(e,k),t') by { RecordHasOpenRecSafe(r,s,e,k); }
               assert GuardedEffectsInvariant(HasAttr(e,k),Effects.singleton(e,k)) by {
-                if model.IsTrueStrong(r,s,HasAttr(e,k)) {
-                  model.IsTrueStrongImpliesIsTrue(r,s,HasAttr(e,k));
+                if IsTrueStrong(r,s,HasAttr(e,k)) {
+                  IsTrueStrongImpliesIsTrue(r,s,HasAttr(e,k));
                   reveal EffectsInvariant();
                 }
               }
             }
           } else {
-            assert model.IsSafe(r,s,e,Type.Record(map[])) by {
+            assert IsSafe(r,s,e,Type.Record(map[])) by {
               assert subty(Type.Record(rt),Type.Record(map[]));
-              model.SubtyCompat(Type.Record(rt),Type.Record(map[]));
-              model.SemSubtyTransport(r,s,e,Type.Record(rt),Type.Record(map[]));
+              SubtyCompat(Type.Record(rt),Type.Record(map[]));
+              SemSubtyTransport(r,s,e,Type.Record(rt),Type.Record(map[]));
             }
-            assert model.IsSafe(r,s,HasAttr(e,k),t') by { model.RecordHasOpenRecSafe(r,s,e,k); }
+            assert IsSafe(r,s,HasAttr(e,k),t') by { RecordHasOpenRecSafe(r,s,e,k); }
           }
         }
         case Entity(et) => {
           assert Typesafe(e,effs,Type.Entity(et)) by { SubtyRefl(Type.Entity(et)); }
-          assert model.IsSafe(r,s,e,Type.Entity(et)) by { Sound(e,Type.Entity(et),effs); }
+          assert IsSafe(r,s,e,Type.Entity(et)) by { Sound(e,Type.Entity(et),effs); }
           if !ets.isAttrPossible(et,k) {
-            model.EntityHasImpossibleFalseSafe(r,s,e,k,et);
+            EntityHasImpossibleFalseSafe(r,s,e,k,et);
           } else {
             var m := ets.getLubRecordType(et).value;
             if k in m {
               if effs.contains(e,k) {
-                assert model.IsSafe(r,s,HasAttr(e,k),t') by {
+                assert IsSafe(r,s,HasAttr(e,k),t') by {
                   reveal EffectsInvariant();
                 }
               } else {
-                assert model.IsSafe(r,s,e,Type.Entity(AnyEntity)) by {
-                  model.SubtyCompat(Type.Entity(et),Type.Entity(AnyEntity));
-                  model.SemSubtyTransport(r,s,e,Type.Entity(et),Type.Entity(AnyEntity));
+                assert IsSafe(r,s,e,Type.Entity(AnyEntity)) by {
+                  SubtyCompat(Type.Entity(et),Type.Entity(AnyEntity));
+                  SemSubtyTransport(r,s,e,Type.Entity(et),Type.Entity(AnyEntity));
                 }
-                assert model.IsSafe(r,s,HasAttr(e,k),t') by { model.EntityHasOpenSafe(r,s,e,k); }
+                assert IsSafe(r,s,HasAttr(e,k),t') by { EntityHasOpenSafe(r,s,e,k); }
                 assert GuardedEffectsInvariant(HasAttr(e,k),Effects.singleton(e,k)) by {
-                  if model.IsTrueStrong(r,s,HasAttr(e,k)) {
-                    model.IsTrueStrongImpliesIsTrue(r,s,HasAttr(e,k));
+                  if IsTrueStrong(r,s,HasAttr(e,k)) {
+                    IsTrueStrongImpliesIsTrue(r,s,HasAttr(e,k));
                     reveal EffectsInvariant();
                   }
                 }
               }
             } else {
-              assert model.IsSafe(r,s,e,Type.Entity(AnyEntity)) by {
-                model.SubtyCompat(Type.Entity(et),Type.Entity(AnyEntity));
-                model.SemSubtyTransport(r,s,e,Type.Entity(et),Type.Entity(AnyEntity));
+              assert IsSafe(r,s,e,Type.Entity(AnyEntity)) by {
+                SubtyCompat(Type.Entity(et),Type.Entity(AnyEntity));
+                SemSubtyTransport(r,s,e,Type.Entity(et),Type.Entity(AnyEntity));
               }
-              assert model.IsSafe(r,s,HasAttr(e,k),t') by { model.EntityHasOpenSafe(r,s,e,k); }
+              assert IsSafe(r,s,HasAttr(e,k),t') by { EntityHasOpenSafe(r,s,e,k); }
             }
           }
         }
       }
-      assert model.IsSafe(r,s,HasAttr(e,k),t) by {
-        model.SubtyCompat(t',t);
-        model.SemSubtyTransport(r,s,HasAttr(e,k),t',t);
+      assert IsSafe(r,s,HasAttr(e,k),t) by {
+        SubtyCompat(t',t);
+        SemSubtyTransport(r,s,HasAttr(e,k),t',t);
       }
     }
 
@@ -1183,7 +1185,7 @@ module validation.thm.soundness {
       requires InstanceOfActionStore(s,acts)
       requires EffectsInvariant(effs)
       requires Typesafe(BinaryApp(BinaryOp.In,e1,e2),effs,t)
-      ensures model.IsSafe(r,s,BinaryApp(BinaryOp.In,e1,e2),t)
+      ensures IsSafe(r,s,BinaryApp(BinaryOp.In,e1,e2),t)
       ensures getEffects(BinaryApp(BinaryOp.In,e1,e2),effs) == Effects.empty()
     {
       var t' :| getType(BinaryApp(BinaryOp.In,e1,e2),effs) == t' && subty(t',t);
@@ -1194,7 +1196,7 @@ module validation.thm.soundness {
       var t1 := getType(e1,effs);
       assert t1.Entity?;
       assert subty(t1,Type.Entity(AnyEntity));
-      assert model.IsSafe(r,s,e1,Type.Entity(AnyEntity)) by { Sound(e1,Type.Entity(AnyEntity),effs); }
+      assert IsSafe(r,s,e1,Type.Entity(AnyEntity)) by { Sound(e1,Type.Entity(AnyEntity),effs); }
 
       assert typechecker.ensureEntitySetType(e2,effs).Ok?;
       var t2 := getType(e2,effs);
@@ -1212,25 +1214,25 @@ module validation.thm.soundness {
       match t' {
         // Easy case
         case Bool(AnyBool) =>
-          assert model.IsSafe(r,s,BinaryApp(BinaryOp.In,e1,e2),Type.Bool(AnyBool)) by {
+          assert IsSafe(r,s,BinaryApp(BinaryOp.In,e1,e2),Type.Bool(AnyBool)) by {
             if e2IsSet {
-              assert model.IsSafe(r,s,e2,Type.Set(Type.Entity(AnyEntity))) by { Sound(e2,Type.Set(Type.Entity(AnyEntity)),effs); }
-              model.InSetSafe(r,s,e1,e2);
+              assert IsSafe(r,s,e2,Type.Set(Type.Entity(AnyEntity))) by { Sound(e2,Type.Set(Type.Entity(AnyEntity)),effs); }
+              InSetSafe(r,s,e1,e2);
             } else {
-              assert model.IsSafe(r,s,e2,Type.Entity(AnyEntity)) by { Sound(e2,Type.Entity(AnyEntity),effs); }
-              model.InSingleSafe(r,s,e1,e2);
+              assert IsSafe(r,s,e2,Type.Entity(AnyEntity)) by { Sound(e2,Type.Entity(AnyEntity),effs); }
+              InSingleSafe(r,s,e1,e2);
             }
           }
         // Harder case: we have to prove that the result is false.
         case Bool(False) =>
           if typechecker.isUnspecifiedVar(e1) && e2IsSpecified {
             UnspecifiedVarHasUnspecifiedEntityType(e1);
-            assert model.IsSafe(r,s,e2,t2) by { Sound(e2,t2,effs); }
+            assert IsSafe(r,s,e2,t2) by { Sound(e2,t2,effs); }
             if e2IsSet {
               var Set(t2e) := t2;
-              model.InSetFalseTypes(r,s,e1,e2,unspecifiedEntityType,t2e);
+              InSetFalseTypes(r,s,e1,e2,unspecifiedEntityType,t2e);
             } else {
-              model.InSingleFalseTypes(r,s,e1,e2,unspecifiedEntityType,t2);
+              InSingleFalseTypes(r,s,e1,e2,unspecifiedEntityType,t2);
             }
           } else {
             match e2 {
@@ -1238,16 +1240,16 @@ module validation.thm.soundness {
                 case Var(v1) =>
                   var et1 :- assert typechecker.getPrincipalOrResource(v1);
                   assert t1 == Type.Entity(EntityLUB({et1}));
-                  assert model.IsSafe(r,s,Var(v1),t1) by { Sound(e1,t1,effs); }
+                  assert IsSafe(r,s,Var(v1),t1) by { Sound(e1,t1,effs); }
                   assert !ets.possibleDescendantOf(et1,u2.ty);
-                  model.InSingleFalseEntityTypeAndLiteral(r,s,e1,et1,u2);
+                  InSingleFalseEntityTypeAndLiteral(r,s,e1,et1,u2);
                 case PrimitiveLit(EntityUID(u1)) =>
                   if isAction(u1.ty) {
                     assert !acts.descendantOf(u1,u2);
                   } else {
                     assert !ets.possibleDescendantOf(u1.ty,u2.ty);
                   }
-                  model.InSingleFalseLiterals(r,s,u1,u2);
+                  InSingleFalseLiterals(r,s,u1,u2);
               }
               case Set(ei2s) =>
                 var euids2 :- assert typechecker.tryGetEUIDs(e2);
@@ -1257,14 +1259,15 @@ module validation.thm.soundness {
                 var eltType :| t2 == Type.Set(eltType);
                 InferSetLemma(e2, ei2s, effs);
                 forall i | 0 <= i < |ei2s|
-                  ensures model.IsSafe(r,s,ei2s[i],Type.Entity(AnyEntity))
+                  ensures IsSafe(r,s,ei2s[i],Type.Entity(AnyEntity))
                 {
                   assert subty(getType(ei2s[i],effs), eltType);
                   SubtyTrans(getType(ei2s[i],effs), eltType, Type.Entity(AnyEntity));
-                  assert model.IsSafe(r,s,ei2s[i],Type.Entity(AnyEntity)) by { Sound(ei2s[i], Type.Entity(AnyEntity), effs); }
+                  assert IsSafe(r,s,ei2s[i],Type.Entity(AnyEntity)) by { Sound(ei2s[i], Type.Entity(AnyEntity), effs); }
                 }
                 forall i | 0 <= i < |ei2s|
-                  ensures model.IsFalse(r,s,BinaryApp(BinaryOp.In,e1,ei2s[i]))
+                  // Note: this is the most expensive part of the proof
+                  ensures IsFalse(r,s,BinaryApp(BinaryOp.In,e1,ei2s[i]))
                 {
                   var u2 :- assert typechecker.tryGetEUID(ei2s[i]);
                   assert u2 in euids2;
@@ -1273,9 +1276,9 @@ module validation.thm.soundness {
                     case Var(v1) =>
                       var et1 :- assert typechecker.getPrincipalOrResource(v1);
                       assert t1 == Type.Entity(EntityLUB({et1}));
-                      assert model.IsSafe(r,s,Var(v1),t1) by { Sound(e1,t1,effs); }
+                      assert IsSafe(r,s,Var(v1),t1) by { Sound(e1,t1,effs); }
                       assert !ets.possibleDescendantOf(et1,u2.ty);
-                      model.InSingleFalseEntityTypeAndLiteral(r,s,e1,et1,u2);
+                      InSingleFalseEntityTypeAndLiteral(r,s,e1,et1,u2);
                     case PrimitiveLit(EntityUID(u1)) =>
                       if isAction(u1.ty) {
                         assert !acts.descendantOfSet(u1,euids2);
@@ -1284,23 +1287,23 @@ module validation.thm.soundness {
                         assert !ets.possibleDescendantOfSet(u1.ty,ets2);
                         assert !ets.possibleDescendantOf(u1.ty,u2.ty);
                       }
-                      model.InSingleFalseLiterals(r,s,u1,u2);
+                      InSingleFalseLiterals(r,s,u1,u2);
                   }
                 }
-                model.InSetFalseIfAllFalse(r,s,e1,ei2s);
+                InSetFalseIfAllFalse(r,s,e1,ei2s);
             }
           }
       }
 
-      assert model.IsSafe(r,s,BinaryApp(BinaryOp.In,e1,e2),t) by {
-        model.SubtyCompat(t',t);
-        model.SemSubtyTransport(r,s,BinaryApp(BinaryOp.In,e1,e2),t',t);
+      assert IsSafe(r,s,BinaryApp(BinaryOp.In,e1,e2),t) by {
+        SubtyCompat(t',t);
+        SemSubtyTransport(r,s,BinaryApp(BinaryOp.In,e1,e2),t',t);
       }
     }
 
     lemma InferCallArgsSound(e: Expr, name: base.Name, args: seq<Expr>, tys: seq<Type>, effs: Effects)
       requires |args| == |tys|
-      requires forall i :: 0 <= i < |args| ==> args[i] < e
+      requires forall i | 0 <= i < |args| :: args[i] < e
       requires Typechecker(ets,acts,reqty).inferCallArgs(e,args,tys,effs).Ok?
       ensures forall i | 0 <= i < |args| :: Typesafe(args[i],effs,tys[i])
     {}
@@ -1312,16 +1315,16 @@ module validation.thm.soundness {
       requires InstanceOfActionStore(s,acts)
       requires EffectsInvariant(effs)
       requires Typesafe(Call(name,es),effs,t)
-      ensures model.IsSafe(r,s,Call(name,es),t)
+      ensures IsSafe(r,s,Call(name,es),t)
       ensures getEffects(Call(name,es),effs) == Effects.empty()
     {
       assert Typechecker(ets,acts,reqty).inferCall(Call(name,es),name,es,effs).Ok?;
       var eft := extFunTypes[name];
       InferCallArgsSound(Call(name,es),name,es,eft.args,effs);
-      forall i | 0 <= i < |es| ensures model.IsSafe(r,s,es[i],eft.args[i]) {
+      forall i | 0 <= i < |es| ensures IsSafe(r,s,es[i],eft.args[i]) {
         Sound(es[i],eft.args[i],effs);
       }
-      model.CallSafe(r,s,name,es);
+      CallSafe(r,s,name,es);
     }
 
     lemma Sound(e: Expr, t: Type, effs: Effects)
@@ -1331,7 +1334,7 @@ module validation.thm.soundness {
       requires InstanceOfActionStore(s,acts)
       requires EffectsInvariant(effs)
       requires Typesafe(e,effs,t)
-      ensures model.IsSafe(r,s,e,t)
+      ensures IsSafe(r,s,e,t)
       ensures GuardedEffectsInvariant(e,getEffects(e,effs))
     {
       assert GuardedEffectsInvariant(e,Effects.empty()) by {
@@ -1369,7 +1372,7 @@ module validation.thm.soundness {
       requires InstanceOfEntityTypeStore(s,ets)
       requires InstanceOfActionStore(s,acts)
       requires Typechecker(ets,acts,reqty).typecheck(e,t).Ok?;
-      ensures model.IsSafe(r,s,e,t)
+      ensures IsSafe(r,s,e,t)
     {
       EmptyEffectsInvariant();
       Sound(e,t,Effects.empty());
