cedar-dafny/thm/slicing.dfy
@@ -24,19 +24,19 @@ module slicing {
 
   ghost predicate isSliceOfPolicyStore(slice: PolicyStore, store: PolicyStore) {
     slice.policies.Keys <= store.policies.Keys &&
-    (forall pid ::
-       pid in slice.policies.Keys ==>
-         slice.policies[pid] == store.policies[pid])
+    (forall pid |
+       pid in slice.policies.Keys ::
+       slice.policies[pid] == store.policies[pid])
   }
 
   ghost predicate isSoundSliceForRequest(request: Request, slice: Store, store: Store) {
     isSliceOfPolicyStore(slice.policies, store.policies) &&
-    (forall pid ::
-       (pid in store.policies.policies.Keys && pid !in slice.policies.policies.Keys) ==>
-         !Authorizer(request, store).satisfied(pid)) &&
-    (forall pid ::
-       pid in slice.policies.policies.Keys ==>
-         Authorizer(request, slice).satisfied(pid) == Authorizer(request, store).satisfied(pid))
+    (forall pid |
+       (pid in store.policies.policies.Keys && pid !in slice.policies.policies.Keys) ::
+       !Authorizer(request, store).satisfied(pid)) &&
+    (forall pid |
+       pid in slice.policies.policies.Keys ::
+       Authorizer(request, slice).satisfied(pid) == Authorizer(request, store).satisfied(pid))
   }
 
   lemma AuthorizationIsCorrectForSoundSlicing(request: Request, slice: Store, store: Store)
